\setlength{\columnsep}{0.1in}

\begin{center}\section*{References}\end{center}

\begin{multicols*}{2}[]

\textbf{Thermodynamics}

Ideal Gas Relationships
\vspace{-1em}
\begin{enumerate}
\item[] Ideal Gas Law \[PV=mRT \]\[ Pv = RT\]\[PV = nR_u T\]
\item[] Compressibility Factor \[Pv = ZRT\]
\item[] Internal Energy of Ideal Gas \[\Delta u = \int_{T_1}^{T_2} c_v(T)dT \approx c_{v,avg}\Delta T\]
\item[] Enthalpy of Ideal Gas \[\Delta h = \int_{T_1}^{T_2} c_p(T)dT \approx c_{p,avg}\Delta T\]
\item[] Entropy of Ideal Gas \[\Delta S_\text{ideal gas} = \underbrace{c_v \ln (T_2 / T_1) + R\ln (V_2 / V_1)}_{c_v\text{ at average temperature}}\]
\[=\underbrace{c_p\ln (T_2 / T_1) - R\ln (P_2 / P_1)}_{c_p\text{ at average temperature}}\]
\end{enumerate}
\vspace{-1em}
Isentropic Ideal Gas Relationships
\vspace{-1em}
\begin{enumerate}
\item[]\[\left(\frac{T_2}{T_1}\right)_{s=\text{const}} = \left(\frac{v_1}{v_2}\right)^{k-1}\]

\item[]\[\left(\frac{T_2}{T_1}\right)_{s=\text{const}} = \left(\frac{P_2}{P_1}\right)^{(k-1)/k}\]

\item[]\[\left(\frac{P_2}{P_1}\right)_{s=\text{const}} = \left(\frac{v_1}{v_2}\right)^{k}\]
\end{enumerate}
\vspace{-1em}
Energy Balances
\vspace{-1em}
\begin{enumerate}
\item[] Nozzle and Diffuser \[\dot m \left(h_1 + \frac{v_1^2}{2}\right) = \dot m \left(h_2 + \frac{v_2^2}{2}\right)\]
\item[] Compressor \[\dot m h_1 + W_\text{in} = \dot m h_2\]
\item[] Pump (liquids only) \[\dot m h_1 + V(P_2-P_1) = \dot m h_2\]
\item[] Turbine \[\dot m h_1 = \dot m h_2 + W_\text{out}\]
\end{enumerate}
Carnot Efficiency
\vspace{-1em}
\begin{enumerate}
\item[] Heat Engine \[\eta = \frac{T_H-T_L}{T_H}\]
\item[] Heat Pump Coefficient of Performance \[\text{COP}_\text{HP} = \frac{T_H}{T_H-T_L}\]
\item[] Refrigerator Coefficient of Performance \[\text{COP}_\text{R} = \frac{T_L}{T_H-T_L}\]
\end{enumerate}
\vspace{-1em}
Heat-Entropy Relationship
\vspace{-1em}
\begin{enumerate}
    \item[] \[\Delta S = \frac{Q}{T_0}\]
    \item[] \[Q = \int_{T_1}^{T_2} TdS\]
\end{enumerate}
\vspace{-1em}
Isentropic Efficiency
\vspace{-1em}
\begin{enumerate}
\item[] Turbine \[\eta = \frac{W_a}{W_s} = \frac{h_1-h_{2a}}{h_1-h_{2s}}\]
\item[] Compressor \[\eta = \frac{W_s}{W_a} = \frac{h_{2s}-h_1}{h_{2a}-h_1} = \underbrace{\frac{V(P_2-P_1)}{h_{2a}-h_1}}_\text{Pumps}\]
\end{enumerate}
\vspace{-1em}
Cycle Efficiency
\vspace{-1em}
\begin{enumerate}
\item[] Otto Cycle \[\eta = 1 - \frac{1}{r^{k-1}}\]
\item[] Diesel Cycle \[\eta = 1 - \frac{1}{r^{k-1}}\left[\frac{r_c^k - 1}{k(r_c-1)}\right]\]
\item[] Brayton Cycle \[\eta = 1 - \frac{1}{r_p^{(k-1)/k}}\]
\item[] Rankine Cycle \[\eta = 1 - \frac{Q_\text{out}}{Q_\text{in}}\]
\item[] Backwork Ratio \[\text{BWR} = \frac{W_\text{in}}{W_\text{out}}\]
\end{enumerate}
\end{multicols*}

\begin{multicols*}{2}[]
\textbf{Statics and Mechanics of Materials}

\vspace{-0.5em}
Stress
\vspace{-0.5em}
\begin{enumerate}
        \item[] Normal Stress \[\sigma_{zz} = \frac{N}{A} + \frac{M_xy}{I_x} - \frac{M_yx}{I_y}\]
        \item[] Shear Stress (average) \[\tau_{zx} = \frac{V_x}{A},\ \tau_{zy} = \frac{V_y}{A}\]
        \item[] Shear Stress due to Torsion \[\tau_{z\theta} = \frac{Tr}{J}\]
\end{enumerate}
\vspace{-0.5em}
Strain
\vspace{-0.5em}
\begin{enumerate}
    \item[] Extensional Strain \[\epsilon = \frac{\sigma}{E} = \frac{\delta}{L_0} \]
    \item[] Shear Strain \[\gamma = \frac{\tau}{G} = \phi_1 + \phi_2\]
    \item[] Multiaxial Hooke's Law 
        \[\epsilon_x = \frac{\sigma_x}{E} - \frac{\nu\sigma_y}{E} - \frac{\nu \sigma_z}{E} + \alpha\Delta T\]
        \[\epsilon_y = \frac{\sigma_y}{E} - \frac{\nu\sigma_x}{E} - \frac{\nu \sigma_z}{E} + \alpha\Delta T\]
        \[\epsilon_z = \frac{\sigma_z}{E} - \frac{\nu\sigma_x}{E} - \frac{\nu \sigma_y}{E} + \alpha\Delta T\]
    \item[] Poisson's Ratio \[E = 2G(1+\nu)\]
\end{enumerate}
\vspace{0.5em}
Extension
\vspace{-0.5em}
\begin{enumerate}
    \item[] Normal Extension \[\delta = \frac{FL_0}{AE}\]
    \item[] Angle of Torsion \[\phi = \frac{TL}{JG}\]
\end{enumerate}
\vspace{-0.5em}
Centroid Locations
\vspace{-1em}
\begin{enumerate}
    \item[] \[A c_x = \sum A_i\overline{x}_i \iff c_x = \frac{\sum A_i\overline{x}_i}{A}\]
    \item[] \[A c_y = \sum A_i\overline{y}_i \iff c_y = \frac{\sum A_i\overline{y}_i}{A}\]
\end{enumerate}
\vspace{20.5em}
Area Moments of Inertia
\vspace{-0.5em}
\begin{enumerate}
    \item[] Parallel Axis Theorem \[I_{x'} = I_x +Ad^2\]
    \item[] Rectangular Section \[I = \frac{1}{12}bh^3\]
    \item[] Circular Section \[I_x = I_y = \frac{\pi r^4}{4} = \frac{\pi d^4}{64}\]
    \item[] Circular Section, Normal Axis \[J = \frac{\pi r^4}{2} = \frac{\pi d^4}{32}\]
\end{enumerate}
\vspace{-1em}
Principle Stress and Stress Transformations
\vspace{-1em}
\begin{enumerate}
    \item[] Stress Transformations \[\sigma_{x'} = \frac{\sigma_x + \sigma_y}{2}+ \frac{\sigma_x - \sigma_y}{2}\cos 2\theta + \tau_{xy}\sin2\theta\]
    \[\sigma_{y'} = \frac{\sigma_x + \sigma_y}{2} - \frac{\sigma_x - \sigma_y}{2}\cos 2\theta - \tau_{xy}\sin2\theta\]
    \[\tau_{x'y'} = -\frac{\sigma_x -\sigma_y}{2}\sin2\theta + \tau_{xy}\cos2\theta\]
    \item[] Principle Stresses \[\sigma_{1,2} = \frac{\sigma_x + \sigma_y}{2} \pm \underbrace{\sqrt{\left(\frac{\sigma_x - \sigma_y}{2}\right)^2 + \tau_{xy}^2}}_{\tau_{\text{max}}}\]
\end{enumerate}
\vspace{-1em}
Principle Strain and Strain Transformations
\vspace{-1em}
\begin{enumerate}
    \item[] Strain Transformations \[\epsilon_{x'} = \frac{\epsilon_x + \epsilon_y}{2} + \frac{\epsilon_x-\epsilon_y}{2}\cos(2\theta) + \frac{\gamma_{xy}}{2}\sin(2\theta)\]
    \[\epsilon_{y'} = \frac{\epsilon_x + \epsilon_y}{2} - \frac{\epsilon_x-\epsilon_y}{2}\cos(2\theta) - \frac{\gamma_{xy}}{2}\sin(2\theta)\]
    \[\frac{\gamma_{x'y'}}{2} = - \frac{\epsilon_x-\epsilon_y}{2}\sin(2\theta) + \frac{\gamma_{xy}}{2}\cos(2\theta)\]
    \item[] Principle Strains \[\epsilon_{1,2} = \frac{\epsilon_x+\epsilon_y}{2}\pm \underbrace{\sqrt{\left(\frac{\epsilon_x-\epsilon_y}{2}\right)^2 + \left(\frac{\gamma_{xy}}{2}\right)^2}}_{\gamma_{\text{max}}/2}\]
    \item[] Strain Gauge Rosette Relationship \[\epsilon_a = \epsilon_x\cos^2\theta_a + \epsilon_y \sin^2\theta_a + \gamma_{xy}\sin\theta_a\cos\theta_a\]
\end{enumerate}
\vspace{-1em}
Bending Deflections
\vspace{-1em}
\begin{enumerate}
    \item[] \[\frac{M}{EI} = \frac{d^2u}{dz^2} = \frac{d\theta}{dz}\]
\end{enumerate}
\end{multicols*}

\textbf{Dynamics and Vibrations}

\begin{multicols*}{2}[]
\vspace{-2em}
Rectilinear Motion
\vspace{-2em}
\begin{enumerate}
    \item[] \[a = v\frac{dv}{ds} \iff ads = vdv\]
\end{enumerate}
\vspace{-1em}
Coordinate Systems
\vspace{-1em}
\begin{enumerate}
    \item[] Polar Coordinates
\vspace{-1em}
    \[\vec{r} = r\hat e_r + z\hat k\]
\vspace{-1em}
    \[\vec{v} = \dot r\hat e_r + r\dot\theta \hat e_\theta + \dot z\hat k\]
\vspace{-1em}
    \[\vec{a} = (\ddot r - r\dot\theta^2)\hat e_r + (r\ddot\theta + 2\dot r\dot\theta)\hat e_\theta + \ddot z\hat k\]
\vspace{-1em}
    \item[] Normal-Tangential Coordinates
\vspace{-1em}
    \[\vec{v} = v\hat e_t\]
\vspace{-1em}
    \[\vec{a} = \dot v\hat e_t + \frac{v^2}{\rho}\hat e_n\]
\end{enumerate}
\vspace{-1em}
Particle Kinetics
\vspace{-1em}
\begin{enumerate}
    \item[] Newton's 2nd Law \[\sum \vec{F} = m\vec{a_c}\]

    \item[] Work-Energy Theorem \[\underbrace{\int_{\vec{R}_1}^{\vec{R}_2} \vec{F}\cdot d\vec{R}}_\text{Work} = \underbrace{T_2-T_1}_\text{Kinetic energy}\]

    \item[] Work-Energy Theorem, Conservative Forces

    \[T_1+V_1+W_\text{nonconservative} = T_2 +V_2\]

    \item[] Impulse-Momentum Equation \[\int_{t_1}^{t_2}\vec{F}dt = m\vec{v}_2 - m\vec{v}_1\]

    \item[] Coefficient of Restitution, rectilinear speeds \[e:=\frac{v_B' - v_A'}{v_A-v_B}\]
\end{enumerate}

Particle Vibrations
\vspace{-1em}
\begin{enumerate}
    \item[] Undamped natural frequency, spring-mass system \[\omega_n = \sqrt\frac{k}{m}\]
    \item[] Equation of Motion, Undamped Vibrations \[\ddot x + \omega_n^2x = 0\]
    \item[] Solution, Undamped Vibrations \[x(t) = x_0\cos(\omega_n t)+ \frac{\dot x_0}{\omega_n}\sin(\omega_n t)\]
    \vspace{-2.5em}
    \item[] Damping ratio, spring-mass damper \[\zeta = \frac{c}{2m\omega_n}\]
    \item[] Damped frequency \[\omega_d = \omega_n\sqrt{1-\zeta^2}\]
    \item[] Equation of Motion, Damped Vibrations \[\ddot x + 2\zeta\omega_n \dot x + \omega_n^2x = 0\]
    \item[] Solution, Damped Vibrations \[x(t) = e^{-\zeta\omega_nt}\left(x_0\cos(\omega_d t)+\frac{\dot x_0+\zeta\omega_nx_0}{\omega_d}\sin(\omega_d t)\right)\]
    \item[] Time Constant ($t=4\tau \implies 98\%$ decay) \[\tau = \frac{1}{\zeta\omega_n}\]
\end{enumerate}

\vspace{-1em}
Planar Rigid Body Kinetics
\vspace{-1em}
\begin{enumerate}
    \item[] General Velocity for Rigid Body (or bodies, points $o$ and $p$) \[\vec{v}_p = \vec{v}_o + \vec{\omega_o}\times\vec{r}_{p/o} + \vec{v}_{p\text{,rel }o}\]
    \item[] General Acceleration for Rigid Body (or bodies, points $o$ and $p$) \[\vec{a}_p = \vec{a}_o + \vec{\alpha}\times\vec{r}_{p/o}+\vec\omega_o\times(\vec{\omega_o}\times\vec{r}_{p/o}) + 2\vec\omega_o \times \vec{v}_{p\text{,rel }o} + \vec{a}_{p\text{,rel }o}\]
    \item[] Parallel Axis Theorem (from center of mass $c$ to point $p$ at distance $d$) \[I_p = I_c + md^2\]
    \item[] Euler's Equation \[\sum M_p = I_p\dot{\vec{\omega}} + \vec{r}_{c/p}\times m\vec{a}_p\]
\end{enumerate}
\vspace{-1em}
Planar Rigid Body Vibrations
\vspace{-1em}
\begin{enumerate}
    \item[] Equation of Motion, Forced Vibrations (with cosine forcing term) \[\ddot x + \frac{c}{m}\dot x + \frac{k}{m}x = \frac{F_0}{m}\cos(\omega_t)\]
    \item[] Tuning Ratio \[\eta = \frac{\omega}{\omega_n}\text{, where }\eta\approx1 \text{ at resonance}\]
    \item[] Steady-State Amplitude of Response, Forced Vibrations \[X = \frac{F_0/k_\text{effective}}{\sqrt{(2\zeta\eta)^2+(1-\eta^2)^2}}\]
    \item[] Steady-State Amplitude of Response, Base Excitations \[X = x_0\sqrt{\frac{1+(2\zeta\eta)^2}{(2\zeta\eta)^2+(1-\eta^2)^2}}\]
\end{enumerate}
\end{multicols*}

\textbf{Fluid Mechanics}
\vspace{-1em}
\begin{center}
\begin{minipage}{\linewidth}
\begin{multicols*}{2}[]
Fluid Properties \begin{enumerate}
\item[] Shear \[\tau = \mu \frac{du}{dy}\]
\item[] Kinematic Viscosity \[\nu = \frac{\mu}{\rho}\]
\end{enumerate}
\vspace{-2em}
Fluid Statics \begin{enumerate}
    \item[] Hydrostatic Equation \[P = P_\text{atm} + \rho g h\]
    \item[] Resultant Force of Hydrostatics \[F_R = \rho gh_cA\]
    \item[] Center of Pressure \[(x_R,\ y_R) = \left(\frac{I_{xy,c}}{Ay_c}+x_c,\ \frac{I_{x,c}}{y_cA}+y_c\right)\]
    \item[] Buoyant Force \[F_b = \rho_\text{fluid}gV_\text{displaced}\]
\end{enumerate}
\vspace{-1em}
Fluid Kinematics
\begin{enumerate}
    \item[] Acceleration of a Fluid \[\vec{a} = \frac{D}{Dt}(\vec{v}) = \frac{\partial \vec{v}}{\partial t} + (\vec{v}\cdot\nabla)\vec{v}\]
    \item[] Streamline Equation \[\frac{dy}{dx} = \frac{v}{u}\]
    \item[] Pathline Equations \[\frac{dx}{dt} = u,\hspace{0.25in}\frac{dy}{dt}=v\]
    \item[] Stream Function \[\frac{\partial \psi}{\partial y} = u,\hspace{0.25in}\frac{\partial\psi}{\partial x} = -v\]
\end{enumerate}
\end{multicols*}
\end{minipage}
\end{center}
\textbf{Bernoulli Equation}
\[P_1 + \frac{1}{2}\rho v_1^2 + \rho gh_1 = P_2 + \frac{1}{2}\rho v_2^2 + \rho gh_2 + \underbrace{\int_{s_1}^{s_2}\frac{\partial v}{\partial t}ds}_\text{neglect if steady}\tag{Unsteady Bernoulli Equation}\]
\vspace{-0.5em}
\textbf{Control Volume Analysis}
\vspace{-1em}
\[\frac{\partial}{\partial t}\int_{CV} \rho dV + \int_{CS}\rho (\vec{v}-\vec{v}_{CV})\cdot\hat{n} dA = 0\tag{Conservation of Mass}\] 
\vspace{-0.5em}
\[\frac{\partial}{\partial t}\int_{CV} \rho \vec{v} dV + \int_{CS} \rho \vec{v}[(\vec{v}-\vec{v}_{CV})\cdot \hat{n}]dA = -\int P \hat{n} dA + \int_{CV}\rho \vec{g} dV + \vec{F}_\text{viscous} +  \vec{F}_\text{ext}\tag{Conservation of Momentum}\]
\[\frac{\partial}{\partial t}\int_{CV} \rho e dV + \int_{CS} \rho e (\vec{v}-\vec{v}_{CV})\cdot \hat{n} dA = \dot Q_\text{net,in} + \dot W_\text{shaft,in} -\int P(\vec{v}-\vec{v}_{CV})\cdot \hat{n} dA\tag{Conservation of Energy}\]
\[\frac{P_\text{out}}{\rho}+\frac{1}{2}v_\text{out}^2 + gz_\text{out} = \frac{P_\text{in}}{\rho} + \frac{1}{2}v_\text{in}^2 + gz_\text{in} + w_\text{shaft,in} - \underbrace{(\hat{u}_\text{out}-\hat{u}_\text{in}-q_\text{net,in})}_\text{losses}\tag{Extended Bernoulli Equation}\]
\textbf{Differential Analysis, Rectangular Coordinates}
\begin{align*}
    \frac{\partial\rho}{\partial t} +\nabla\cdot (\rho\vec{v}) = 0\ \xrightarrow[]{\text{if incompressible}}& \ \nabla\cdot\vec{v}:=\frac{\partial u}{\partial x}+\frac{\partial v}{\partial y}+\frac{\partial w}{\partial z} = 0\tag{Continuity}\\
    \frac{\partial u}{\partial t} + u \frac{\partial u}{\partial x} + v\frac{\partial u}{\partial y} + w\frac{\partial u}{\partial z} &= -\frac{1}{\rho}\frac{\partial p}{\partial x} + \nu\left(\frac{\partial^2 u}{\partial x^2} + \frac{\partial^2 u}{\partial y^2} + \frac{\partial^2 u}{\partial z^2}\right) + g_x\tag{$x$}\\
    \frac{\partial v}{\partial t} + u \frac{\partial v}{\partial x} + v\frac{\partial v}{\partial y} + w\frac{\partial v}{\partial z} &= -\frac{1}{\rho}\frac{\partial p}{\partial y} + \nu\left(\frac{\partial^2 v}{\partial x^2} + \frac{\partial^2 v}{\partial y^2} + \frac{\partial^2 v}{\partial z^2}\right) + g_y\tag{$y$}\\
    \frac{\partial w}{\partial t} + u \frac{\partial w}{\partial x} + v\frac{\partial w}{\partial y} + w\frac{\partial w}{\partial z} &= -\frac{1}{\rho}\frac{\partial p}{\partial z} + \nu\left(\frac{\partial^2 w}{\partial x^2} + \frac{\partial^2 w}{\partial y^2} + \frac{\partial^2 w}{\partial z^2}\right) + g_z\tag{$z$}
\end{align*}
\textbf{Differential Analysis, Polar Coordinates}
\begin{align*}
    \frac{1}{r}\frac{\partial}{\partial r}(rv_r) + \frac{1}{r}\frac{\partial v_\theta}{\partial\theta} + \frac{\partial v_z}{\partial z} &= 0\tag{Incompressible Continuity}\\
    \rho\left(\frac{\partial v_r}{\partial t} + v_r \frac{\partial v_r}{\partial r} + \frac{v_\theta}{r}\frac{\partial v_r}{\partial \theta} - \frac{v_\theta^2}{r} + v_z \frac{\partial v_r}{\partial z}\right) &= -\frac{\partial p}{\partial r}+\mu \left[\frac{1}{r}\frac{\partial}{\partial r} \left(r \frac{\partial v_r}{\partial r}\right) - \frac{v_r}{r^2} + \frac{1}{r^2} \frac{\partial^2 v_r}{\partial \theta^2} - \frac{2}{r^2}\frac{\partial v_\theta}{\partial \theta} + \frac{\partial^2 v_r}{\partial z^2}\right] + \rho g_r\tag{$r$}\\
    \rho\left(\frac{\partial v_\theta}{\partial t} 
    + v_r \frac{\partial v_\theta}{\partial r} 
    + \frac{v_\theta}{r}\frac{\partial v_\theta}{\partial \theta} 
    + \frac{v_\theta v_r}{r} + v_z \frac{\partial v_\theta}{\partial z}\right) 
    &= -\frac{1}{r}\frac{\partial p}{\partial\theta} + \mu \left[\frac{1}{r}\frac{\partial}{\partial r} \left(r \frac{\partial v_\theta}{\partial r}\right) 
    - \frac{v_\theta}{r^2} 
    + \frac{1}{r^2} \frac{\partial^2 v_\theta}{\partial \theta^2} 
    + \frac{2}{r^2}\frac{\partial v_r}{\partial \theta} 
    + \frac{\partial^2 v_\theta}{\partial z^2}\right] + \rho g_\theta\tag{$\theta$}\\
        \rho\left(\frac{\partial v_z}{\partial t} + v_r\frac{\partial v_z}{\partial r} + \frac{v_\theta}{r}\frac{\partial v_z}{\partial \theta} + v_z\frac{\partial v_z}{\partial \theta}\right) &= -\frac{\partial p}{\partial z} + \mu\left[\frac{1}{r}\frac{\partial}{\partial r}\left(r\frac{\partial v_z}{\partial r}\right) + \frac{1}{r^2}\frac{\partial^2 v_z}{\partial\theta^2} + \frac{\partial^2 v_z}{\partial z^2}\right] + \rho g_z\tag{$z$}
\end{align*}